wip: add nat_to_intseq_le[be] and lemmas

code/experimental/curve25519/Hacl.Impl.Curve25519.Generic.fst
@@ -128,9 +128,14 @@ let encode_point_ #s o i =
   assert (feval h1 tmp == S.fmul (S.fpow (feval h0 z) (pow2 255 - 21)) (feval h0 x));
   assert (feval h1 tmp == S.fmul (feval h0 x) (S.fpow (feval h0 z) (pow2 255 - 21)));
   store_felem u64s tmp;
-  uints_to_bytes_le #U64 4ul o u64s;
   let h2 = ST.get () in
-  assume (as_seq h2 o == BSeq.nat_to_bytes_le 32 (feval h1 tmp));
+  assert (BSeq.nat_from_intseq_le (as_seq h2 u64s) == feval h1 tmp);
+  Hacl.Impl.Curve25519.Lemmas.lemma_nat_to_uints64_le_4 (as_seq h2 u64s) (feval h1 tmp);
+  assert (as_seq h2 u64s == BSeq.nat_to_intseq_le 4 (feval h1 tmp));
+  uints_to_bytes_le #U64 4ul o u64s;
+  let h3 = ST.get () in
+  BSeq.uints_to_bytes_le_nat_lemma #U64 #SEC 4 (feval h1 tmp);
+  assert (as_seq h3 o == BSeq.nat_to_bytes_le 32 (feval h1 tmp));
   pop_frame()
 
 (* WRAPPER to Prevent Inlining *)
