code/experimental/curve25519/Hacl.Impl.Curve25519.Lemmas.fst
@@ -16,3 +16,7 @@ let lemma_nat_from_uints64_le_4 b =
   assert (nat_from_intseq_le_ (Seq.slice b 2 4) == v b.[2] + pow2 64 * (nat_from_intseq_le_ (Seq.slice b 3 4)));
   assert (nat_from_intseq_le_ (Seq.slice b 3 4) == v b.[3]);
   assert (res == v b.[0] + pow2 64 * (v b.[1] + pow2 64 * (v b.[2] + pow2 64 * v b.[3])))
+
+let lemma_nat_to_uints64_le_4 b n =
+  let b1 = nat_to_intseq_le 4 n in
+  nat_from_intseq_le_inj b1 b
