lib/fst/Lib.ByteSequence.fst
@@ -116,43 +116,48 @@ let nat_from_bytes_le = nat_from_intseq_le #U8
 
 #set-options "--max_fuel 1"
 
-val nat_to_bytes_be_:
-    #l:secrecy_level
+val nat_to_intseq_be_:
+    #t:inttype -> #l:secrecy_level
   -> len:nat
-  -> n:nat{ n < pow2 (8 * len)}
-  -> Tot (b:bytes_l l {length b == len /\ n == nat_from_intseq_be #U8 b}) (decreases len)
-let rec nat_to_bytes_be_ #l len n =
-  if len = 0 then create len (uint #U8 #l 0)
+  -> n:nat{n < pow2 (bits t * len)}
+  -> Tot (b:seq (uint_t t l){length b == len /\ n == nat_from_intseq_be b}) (decreases len)
+let rec nat_to_intseq_be_ #t #l len n =
+  if len = 0 then create len (uint #t #l 0)
   else
     let len' = len - 1 in
-    let byte = uint #U8 #l (n % 256) in
-    let n' = n / 256 in
-    Math.Lemmas.pow2_plus 8 (8 * len');
-    let b' = nat_to_bytes_be_ len' n' in
-    let b  = Seq.append b' (create 1 byte) in
-    Seq.append_slices b' (create 1 byte);
+    let tt = uint #t #l (n % modulus t) in
+    let n' = n / modulus t in
+    assert (modulus t = pow2 (bits t));
+    FStar.Math.Lemmas.lemma_div_lt_nat n (bits t * len) (bits t);
+    let b' = nat_to_intseq_be_ len' n' in
+    let b  = Seq.append b' (create 1 tt) in
+    Seq.append_slices b' (create 1 tt);
     b
 
-let nat_to_bytes_be = nat_to_bytes_be_
+let nat_to_intseq_be = nat_to_intseq_be_
 
-val nat_to_bytes_le_:
-    #l:secrecy_level
+val nat_to_intseq_le_:
+    #t:inttype -> #l:secrecy_level
   -> len:nat
-  -> n:nat{n < pow2 (8 * len)}
-  -> Tot (b:bytes_l l {length b == len /\ n == nat_from_intseq_le b}) (decreases len)
-let rec nat_to_bytes_le_ #l len n =
-  if len = 0 then create len (uint #U8 #l 0)
+  -> n:nat{n < pow2 (bits t * len)}
+  -> Tot (b:seq (uint_t t l){length b == len /\ n == nat_from_intseq_le b}) (decreases len)
+let rec nat_to_intseq_le_ #t #l len n =
+  if len = 0 then create len (uint #t #l 0)
   else
     let len' = len - 1 in
-    let byte = uint #U8 #l (n % 256) in
-    let n' = n / 256 in
-    Math.Lemmas.pow2_plus 8 (8 * len');
-    let b' = nat_to_bytes_le_ #l len' n' in
-    let b = Seq.append (create 1 byte) b' in
-    Seq.append_slices (create 1 byte) b';
+    let tt = uint #t #l (n % modulus t) in
+    let n' = n / modulus t in
+    assert (modulus t = pow2 (bits t));
+    FStar.Math.Lemmas.lemma_div_lt_nat n (bits t * len) (bits t);
+    let b' = nat_to_intseq_le_ len' n' in
+    let b = Seq.append (create 1 tt) b' in
+    Seq.append_slices (create 1 tt) b';
     b
 
-let nat_to_bytes_le = nat_to_bytes_le_
+let nat_to_intseq_le = nat_to_intseq_le_
+
+let nat_to_bytes_be = nat_to_intseq_be_ #U8
+let nat_to_bytes_le = nat_to_intseq_le_ #U8
 
 val index_nat_to_bytes_le:
     #l:secrecy_level
@@ -321,10 +326,10 @@ let uints_from_bytes_le_nat_lemma0 #t #l #len b =
   assert (nat_from_intseq_le_ (Seq.slice b 0 (numbytes t)) == v r.[0])
 
 val uints_from_bytes_le_nat_lemma_:
-    #t:inttype{~(t == U1)} 
-  -> #l:secrecy_level 
+    #t:inttype{~(t == U1)}
+  -> #l:secrecy_level
   -> #len:size_nat{len * numbytes t < pow2 32}
-  -> b:lbytes_l l (len * numbytes t) -> 
+  -> b:lbytes_l l (len * numbytes t) ->
   Lemma (nat_from_intseq_le_ (uints_from_bytes_le #t #l #len b) == nat_from_intseq_le_ b)
 let rec uints_from_bytes_le_nat_lemma_ #t #l #len b =
   if len = 0 then ()
@@ -336,3 +341,14 @@ let rec uints_from_bytes_le_nat_lemma_ #t #l #len b =
   end
 
 let uints_from_bytes_le_nat_lemma #t #l #len b = uints_from_bytes_le_nat_lemma_ #t #l #len b
+
+let uints_to_bytes_le_nat_lemma #t #l len n = admit()
+
+let rec nat_from_intseq_le_inj #t #l b1 b2 =
+  if length b1 = 0 then ()
+  else begin
+    nat_from_intseq_le_inj (Seq.slice b1 1 (length b1)) (Seq.slice b2 1 (length b2));
+    Seq.lemma_split b1 1;
+    Seq.lemma_split b2 1;
+    uintv_extensionality (Seq.index b1 0) (Seq.index b2 0)
+  end
